Resolution Inferenzregeln

Ground_Order_Resolution_Lifting.thy
@@ -1,58 +1,38 @@
 theory Ground_Order_Resolution_Lifting
   imports
     Ground_Order_Resolution
+    Abstract_Substitution.Functional_Substitution
+    Abstract_Substitution.Functional_Substitution_Lifting
+    Typing
 begin
 
 type_synonym 'f ground_atom = "'f gterm uprod"
 type_synonym ('f, 'v) atom = "('f, 'v) term uprod"
 
-locale grounding_lifting =
-  functional_substitution_lifting where sub_vars = sub_vars and sub_subst = sub_subst and
-  map = map +
-  sub: grounding where vars = sub_vars and subst = sub_subst and to_ground = sub_to_ground and
-  from_ground = sub_from_ground +
-  natural_functor_conversion where map = map and map_to = to_ground_map and
-  map_from = from_ground_map and map' = ground_map and to_set' = to_set_ground
-  for
-    sub_to_ground :: "'sub \<Rightarrow> 'sub\<^sub>G" and
-    sub_from_ground :: "'sub\<^sub>G \<Rightarrow> 'sub" and
-    sub_vars :: "'sub \<Rightarrow> 'var set" and
-    sub_subst :: "'sub \<Rightarrow> ('var \<Rightarrow> 'base) \<Rightarrow> 'sub" and
-    map :: "('sub \<Rightarrow> 'sub) \<Rightarrow> 'expr \<Rightarrow> 'expr" and
-    to_ground_map :: "('sub \<Rightarrow> 'sub\<^sub>G) \<Rightarrow> 'expr \<Rightarrow> 'expr\<^sub>G" and
-    from_ground_map :: "('sub\<^sub>G \<Rightarrow> 'sub) \<Rightarrow> 'expr\<^sub>G \<Rightarrow> 'expr" and
-    ground_map :: "('sub\<^sub>G \<Rightarrow> 'sub\<^sub>G) \<Rightarrow> 'expr\<^sub>G \<Rightarrow> 'expr\<^sub>G" and
-    to_set_ground :: "'expr\<^sub>G \<Rightarrow> 'sub\<^sub>G set"
-begin
-
-definition to_ground :: "'expr \<Rightarrow> 'expr\<^sub>G" where
-  "to_ground expr \<equiv> to_ground_map sub_to_ground expr"
-
-end
 
 context ground_order_resolution_calculus
 begin
 
-lemma (in grounding_lifting) resolution_lifting:
+lemma resolution_lifting:
   fixes
-    D\<^sub>G C\<^sub>G :: "'f gterm clause" and
+    D\<^sub>G C\<^sub>G :: "'f ground_atom clause" and
     D C :: "('f, 'v) atom clause" and
     \<gamma> :: "('f, 'v) subst"
   defines
-    D\<^sub>G [simp]: "D\<^sub>G \<equiv> to_ground (D \<cdot> \<gamma>)" and
-    C\<^sub>G [simp]: "C\<^sub>G \<equiv> to_ground (C \<cdot> \<gamma>)"
+    D\<^sub>G [simp]: "D\<^sub>G \<equiv> grounding_lifting.to_ground (functional_substitution_lifting.subst D \<gamma>)" and
+    C\<^sub>G [simp]: "C\<^sub>G \<equiv> grounding_lifting.to_ground (functional_substitution_lifting.subst C \<gamma>)"
   assumes
     ground_resolution: "ground_order_resolution_calculus.resolution D\<^sub>G C\<^sub>G" and
-    D_grounding: "is_ground (D \<cdot> \<gamma>)" and 
-    C_grounding: "is_ground (C \<cdot> \<gamma>)" and
-    select: "from_ground (select\<^sub>G D\<^sub>G) = (select D) \<cdot> \<gamma>" and
-    D_is_welltyped: "is_welltyped \<V> D" and
+    D_grounding: "functional_substitution.is_ground (functional_substitution_lifting.subst D \<gamma>)" and 
+    C_grounding: "functional_substitution.is_ground (functional_substitution_lifting.subst C \<gamma>)" and
+    select: "grounding_lifting.from_ground (select\<^sub>G D\<^sub>G) = functional_substitution_lifting.subst (select D) \<gamma>" and
+    D_is_welltyped: "typing_lifting.is_welltyped \<V> D" and
     \<gamma>_is_welltyped: "is_welltyped_on (vars D) \<V> \<gamma>" and
     \<V>: "infinite_variables_per_type \<V>"
   obtains C'
   where
-    "eq_resolution (D, \<V>) (C', \<V>)"
+    "resolution (D, \<V>) (C', \<V>)"
     "Infer [D\<^sub>G] C\<^sub>G \<in> inference_groundings (Infer [(D, \<V>)] (C', \<V>))"
-    "C' \<cdot> \<gamma> = C \<cdot> \<gamma>"
+    "functional_substitution_lifting.subst C' \<gamma> = functional_substitution_lifting.subst C  \<gamma>"
   using ground_resolution
 end
