ROOT~
@@ -3,8 +3,10 @@ session Ordered_Resolution = Saturation_Framework_Extensions +
     First_Order_Clause
     Saturation_Framework
     Saturation_Framework_Extensions
+    Abstract_Substitution
 
 theories (* These theories contain the main results. *)
     Ground_Order_Resolution_Completeness
     Ground_Order_Resolution_Soundness
     Ground_Order_Resolution
+    Ground_Order_Resolution_Lifting
